CertifyingDatalog/Parsing.lean
@@ -1,7 +1,7 @@
 import Std.Data.List.Basic
 import CertifyingDatalog.Datalog
-import Lean.Data.Json.FromToJson
 import CertifyingDatalog.Basic
+import Lean.Data.Json.FromToJson
 
 def tokenizeHelper (s: List Char) (currToken: Option String) (tokens: List String): List String :=
   match s with
@@ -27,240 +27,184 @@ def tokenizeHelper (s: List Char) (currToken: Option String) (tokens: List Strin
 
 def tokenize (s: String): List String := tokenizeHelper s.data Option.none List.nil
 
-def listStringToString (l: List String): String :=
-  List.foldl (fun (x y: String) => x ++ "," ++ y) "" l
+inductive mockTerm
+| constant: String → mockTerm
+| variable: String → mockTerm
+deriving DecidableEq, Lean.FromJson, Lean.ToJson, Repr
+
+def mockTerm.toString (mt: mockTerm): String :=
+  match mt with
+  | mockTerm.constant c => "constant " ++ c
+  | mockTerm.variable v => "variable " ++ v
+
+--#eval Lean.toJson (mockTerm.constant "b")
 
 structure mockAtom where
-  symbol: String
-  terms: List (String)
-deriving Repr, DecidableEq
+  (symbol: String)
+  (terms: List mockTerm)
+deriving DecidableEq, Lean.FromJson, Lean.ToJson, Repr
 
-def mockAtom.toString (ma: mockAtom) := ma.symbol ++ "(" ++ (listStringToString ma.terms) ++ ")"
+--#eval Lean.toJson (mockAtom.mk "R" [mockTerm.constant "c", mockTerm.variable "v"])
 
 structure mockRule where
   head: mockAtom
   body: List (mockAtom)
-deriving Repr, DecidableEq
+deriving Repr, DecidableEq, Lean.FromJson, Lean.ToJson
 
-def mockRule.toString (mr: mockRule) := mr.head.toString ++ " :- " ++ listStringToString (List.map mockAtom.toString mr.body)
+inductive jsonTree
+| node (label: String) (children: List jsonTree)
+deriving Repr, Lean.ToJson, Lean.FromJson
 
-def findArity (symbol: String) (relationList: List (String × Nat)): Option Nat :=
-  match relationList with
-  | [] => Option.none
-  | (a,b)::tl =>
-    if symbol == a
-    then Option.some b
-    else findArity symbol tl
+structure problemInput where
+  (trees: List jsonTree)
+  (program: List (mockRule))
+  (completion: Bool)
+deriving Repr, Lean.FromJson, Lean.ToJson
 
-def parseMockAtomFromStack (relationList: List (String × Nat)) (stack: List String): Except String (mockAtom × List (String × Nat)) :=
-  match stack with
-  | [] => Except.error "Can't parse an atom from an empty stack"
-  | hd::tl =>
-    let arity:= findArity hd relationList
-    match arity with
-    | Option.some a =>
-      if tl.length == a
-      then Except.ok ({symbol:= hd, terms:= tl}, relationList)
-      else Except.error ("Relation symbol " ++ hd ++ "occurs multiple times with different arity")
-    | Option.none =>
-      Except.ok ({symbol:= hd, terms:= tl}, relationList.insert (hd, tl.length))
+structure parsingArityHelper where
+  (relationList: List String)
+  (arity: {x // x ∈ relationList} → Nat)
 
-def parseMockAtom.go (relationList: List (String × Nat)) (l: List String) (stack: List String): Except String (mockAtom × List (String × Nat)) :=
-  match l with
-  | [] => Except.error "No closing bracket"
-  | hd::tl =>
-    if hd == ")"
-    then
-      if tl.isEmpty
-      then parseMockAtomFromStack relationList stack
-      else
-        if tl = ["."]
-        then parseMockAtomFromStack relationList stack
-        else Except.error ("Symbols after closing bracket" ++ listStringToString tl)
-    else
-      if hd == "("
-      then parseMockAtom.go relationList tl stack
-      else parseMockAtom.go relationList tl (stack.concat hd)
+def emptyParsingArityHelper: parsingArityHelper := {relationList:= [], arity:= fun _ => 0}
 
-def parseMockAtom (relationList: List (String × Nat)) (l: List String): Except String (mockAtom × List (String × Nat)) :=
-  match parseMockAtom.go relationList l [] with
-  | Except.ok x => Except.ok x
-  | Except.error msg => Except.error ("Error parsing" ++ (List.foldl (fun (x y: String) => x ++ y) "" l) ++ msg)
-
-
-
-def parseMockAtomList.go (relationList: List (String × Nat)) (l: List String) (stack: List String) (curr: List mockAtom): Except String (List mockAtom × List (String × Nat)) :=
-  match l with
-  | [] =>
-    if stack.isEmpty ∨ stack == ["."]
-    then Except.ok (curr, relationList)
-    else Except.error "No closing bracket"
-  | hd :: tl =>
-    if hd == ")"
-    then
-      match parseMockAtomFromStack relationList stack with
-      | Except.error msg => Except.error msg
-      | Except.ok (atom, relationList') =>
-        parseMockAtomList.go relationList' tl [] (curr.concat atom)
-    else
-      if hd == "("
-      then parseMockAtomList.go relationList tl stack curr
-      else parseMockAtomList.go relationList tl (stack.concat hd) curr
-
-def parseMockAtomList (relationList: List (String × Nat)) (l: List String): Except String (List mockAtom × List (String × Nat)) := parseMockAtomList.go relationList l [] []
-
-def parseMockRule (relationList: List (String × Nat)) (l: List String): Except String (mockRule × List (String × Nat )) :=
-  match l with
-  | [] => Except.error "Cannot parse a rule from a empty String"
-  | hd::tl =>
-  let splitResult := List.splitOn ":-" (hd::tl)
-    if h: splitResult.length = 1
-    then
-      have p: 0 < splitResult.length := by
-        simp [h]
-      match parseMockAtom relationList (splitResult.get (Fin.mk 0 p)) with
-      | Except.error msg => Except.error msg
-      | Except.ok (atom, relationList') =>
-        Except.ok ({head:= atom, body:= []}, relationList')
-    else
-      if h:splitResult.length = 2
-      then
-        have p: 0 < splitResult.length := by
-          simp [h]
-        have q: 1 < splitResult.length := by
-          simp [h]
-        match parseMockAtom relationList (splitResult.get (Fin.mk 0 p)) with
-        | Except.error msg => Except.error msg
-        | Except.ok (head, relationList') =>
-          match parseMockAtomList relationList' (splitResult.get (Fin.mk 1 q)) with
-          | Except.error msg => Except.error msg
-          | Except.ok (body, relationList'') =>
-            Except.ok ({head:= head, body:= body}, relationList'')
-      else Except.error "Too many occurences of :-"
-
-def extendFunctionFromList {A B: Type} [DecidableEq A] (l1 l2: List (A × B)) (f: {x: A // x ∈ Prod.fst (List.unzip l2) } → B) : {x: A // x ∈ Prod.fst (List.unzip l2) } → B :=
-  match l1 with
-  | List.nil => f
-  | (a,b)::tl => extendFunctionFromList tl l2 (fun (x: { y // y ∈ Prod.fst (List.unzip l2) })  => if (x.val = a )then b else f x)
-
-def parsingSignature (relationList: List (String × Nat )): signature := {constants:= {x: String // ¬ x.startsWith "?"}, vars := {x: String // x.startsWith "?"}, relationSymbols := {x: String // x ∈ Prod.fst (List.unzip relationList)}, relationArity := extendFunctionFromList relationList relationList (fun _ => 0)}
-
-instance (relationList: List (String × Nat )): DecidableEq (parsingSignature relationList).constants := Subtype.instDecidableEqSubtype
-
-instance (relationList: List (String × Nat )): Nonempty (parsingSignature relationList).constants := by
-  use ""
-  simp
-
-
-instance (relationList: List (String × Nat )): DecidableEq (parsingSignature relationList).vars := Subtype.instDecidableEqSubtype
-
-instance (relationList: List (String × Nat )): DecidableEq (parsingSignature relationList).relationSymbols := Subtype.instDecidableEqSubtype
-
-def parseConstantFromString (relationList: List (String × Nat)) (s: String): Except String (parsingSignature relationList).constants :=
-  if p: s.startsWith "?"
-  then Except.error "Constants are not allowed to start with a ?"
-  else Except.ok (Subtype.mk s p)
-
-def parseTermFromString (relationList: List (String × Nat)) (s: String): term (parsingSignature relationList) :=
-  if p: s.startsWith "?"
-  then (term.variableDL (Subtype.mk s p))
-  else (term.constant (Subtype.mk s p))
-
-def mockAtom.toAtom (ma: mockAtom) (relationList: List (String × Nat)): Except String (atom (parsingSignature relationList)) :=
-  if p: ma.symbol ∈ Prod.fst (List.unzip relationList)
+def extendParsingArityHelper (sig: parsingArityHelper) (symbol: String) (arity: Nat): Except String parsingArityHelper :=
+  if h: symbol ∈ sig.relationList
   then
-    if h: (parsingSignature relationList).relationArity (Subtype.mk ma.symbol p) = ma.terms.length
+    if sig.arity (Subtype.mk symbol h) == arity
     then
-      have h': List.length (List.map (parseTermFromString relationList) ma.terms) = signature.relationArity (parsingSignature relationList) { val := ma.symbol, property := p } := by
-        rw [List.length_map, ← h]
-      Except.ok {symbol := (Subtype.mk ma.symbol p), atom_terms := List.map (parseTermFromString relationList) ma.terms, term_length := h' }
+      Except.ok sig
     else
-      Except.error ("Number of atom terms does not match arity for " ++ ma.toString)
+      Except.error ("Mismatched arity for " ++ symbol ++ " Given ")
   else
-    Except.error ("Unknown symbol" ++ ma.symbol)
+    Except.ok {relationList := sig.relationList ++ [symbol], arity := (fun x => if q:(x = symbol) then arity else
+      have p: x.val ∈ sig.relationList := by
+        have h': x.val ∈ (sig.relationList ++ [symbol] )
+        apply x.property
+        simp at h'
+        cases h' with
+        | inl h' =>
+          apply h'
+        | inr h' =>
+          exact absurd h' q
 
+     sig.arity (Subtype.mk x.val p))}
 
-def mockRule.toRule (mr: mockRule) (relationList: List (String × Nat)): Except String (rule (parsingSignature relationList)) :=
-  match mr.head.toAtom  relationList with
-  | Except.error msg => Except.error ("Error parsing " ++ mr.toString ++ " -- " ++ msg)
+def parsingSignature (helper: parsingArityHelper): signature :=
+  {constants:= String, vars:= String, relationSymbols := {x // x ∈ helper.relationList}, relationArity := helper.arity}
+
+instance (helper: parsingArityHelper): DecidableEq (parsingSignature helper).constants :=
+by
+  unfold parsingSignature
+  simp
+  apply instDecidableEqString
+
+instance (helper: parsingArityHelper): Nonempty (parsingSignature helper).constants :=
+by
+  unfold parsingSignature
+  simp
+  use ['a']
+
+instance (helper: parsingArityHelper): DecidableEq (parsingSignature helper).vars :=
+by
+  unfold parsingSignature
+  simp
+  apply instDecidableEqString
+
+instance (helper: parsingArityHelper): DecidableEq (parsingSignature helper).relationSymbols :=  Subtype.instDecidableEqSubtype
+
+def getArityHelperFromMockAtom (helper: parsingArityHelper) (ma: mockAtom): Except String parsingArityHelper := extendParsingArityHelper helper ma.symbol (ma.terms.length)
+
+def getArityHelperFromMockAtomList (helper: parsingArityHelper) (l: List mockAtom): Except String parsingArityHelper :=
+  match l with
+  | [] => Except.ok helper
+  | hd::tl =>
+    match getArityHelperFromMockAtom helper hd with
+    | Except.error e => Except.error e
+    | Except.ok newHelper =>
+      getArityHelperFromMockAtomList newHelper tl
+
+def getArityHelperFromMockRule (helper: parsingArityHelper) (mr: mockRule): Except String parsingArityHelper :=
+  match getArityHelperFromMockAtom helper mr.head with
+  | Except.error e => Except.error e
+  | Except.ok newHelper => getArityHelperFromMockAtomList newHelper mr.body
+
+def getArityHelperFromProgram.go (helper: parsingArityHelper) (l: List mockRule): Except String parsingArityHelper :=
+  match l with
+  | [] => Except.ok helper
+  | hd::tl =>
+    match getArityHelperFromMockRule helper hd with
+    | Except.error e => Except.error e
+    | Except.ok newHelper => getArityHelperFromProgram.go newHelper tl
+
+def getArityHelperFromProgram (l: List mockRule): Except String parsingArityHelper := getArityHelperFromProgram.go emptyParsingArityHelper l
+
+def transformMockTermToTerm (helper: parsingArityHelper) (mt: mockTerm): term (parsingSignature helper) :=
+  match mt with
+  | mockTerm.constant c => term.constant c
+  | mockTerm.variable v => term.variableDL v
+
+def transformMockAtomToAtom (helper: parsingArityHelper) (ma: mockAtom): Except String (atom (parsingSignature helper)) :=
+  if h: ma.symbol ∈ helper.relationList
+  then
+    if p: helper.arity (Subtype.mk ma.symbol h) = ma.terms.length
+    then
+      have q: List.length (List.map (transformMockTermToTerm helper) ma.terms) =
+    signature.relationArity (parsingSignature helper) { val := ma.symbol, property := h } := by
+        rw [List.length_map]
+        rw [← p]
+        unfold parsingSignature
+        simp
+
+    Except.ok {symbol := (Subtype.mk ma.symbol h), atom_terms := List.map (transformMockTermToTerm helper) ma.terms, term_length := q}
+    else Except.error ("Wrong arity for " ++ ma.symbol)
+  else Except.error ("Unknown symbol" ++ ma.symbol)
+
+def transformMockRuleToRule (helper: parsingArityHelper) (mr: mockRule): Except String (rule (parsingSignature helper)) :=
+  match transformMockAtomToAtom helper mr.head with
+  | Except.error e => Except.error e
   | Except.ok head =>
-    match List.map_except (fun x => mockAtom.toAtom x relationList) mr.body with
-    | Except.error msg => Except.error ("Error parsing " ++ mr.toString ++ " -- " ++ msg)
+    match List.map_except (transformMockAtomToAtom helper) mr.body with
+    | Except.error e => Except.error e
     | Except.ok body => Except.ok {head:= head, body:= body}
 
 
-def parseMockProgram.go (relationList: List (String × Nat)) (l: List String) (currProgram: List mockRule): Except String ((List mockRule) × List (String × Nat)) :=
-  match l with
-  | [] => Except.ok (currProgram, relationList)
-  | hd::tl =>
-    -- ignore empty lines or declarations
-    if hd.startsWith "@" ∨ hd = ""
-    then parseMockProgram.go relationList tl currProgram
-    else
-      match parseMockRule relationList (tokenize hd) with
-      | Except.error msg => Except.error ("Error parsing " ++ hd ++ " -- " ++ msg)
-      | Except.ok (r, relationList') => parseMockProgram.go relationList' tl (currProgram.concat r)
-
-def parseMockProgram (l: List String): Except String ((List mockRule) × List (String × Nat)) := parseMockProgram.go [] l []
-
-def mockProgramToProgram.go (p: List mockRule) (relationList: List (String × Nat)) (curr: List (rule (parsingSignature relationList))): Except String (List (rule (parsingSignature relationList))) :=
-  match p with
-  | [] => Except.ok curr
-  | hd::tl =>
-    match hd.toRule relationList with
-    | Except.error msg => Except.error msg
-    | Except.ok r => mockProgramToProgram.go tl relationList (curr.concat r)
-
-def mockProgramToProgram (p: List mockRule) (relationList: List (String × Nat)): Except String (List (rule (parsingSignature relationList))) :=
-  mockProgramToProgram.go p relationList []
-
-
-inductive Tree
-| node (label: String) (children: List Tree): Tree
-deriving Repr, Lean.ToJson, Lean.FromJson
-
-
-
-def parseGroundAtomFromStack (relationList: List (String × Nat)) (stack: List String): Except String (groundAtom (parsingSignature relationList)) :=
+def parseGroundAtomFromStack (helper: parsingArityHelper) (stack: List String): Except String (groundAtom (parsingSignature helper)) :=
   match stack with
-  | List.nil => Except.error "Cannot parse an atom from an empty stack"
+  | [] => Except.error "Can't parse ground atom from empty string"
   | hd::tl =>
-    if h:hd ∈ Prod.fst (List.unzip relationList)
+    if h: hd ∈  helper.relationList
     then
-      let terms := List.map_except (fun x => parseConstantFromString relationList x) tl
-      match terms with
-      | Except.ok l =>
-        if p: l.length = (parsingSignature relationList).relationArity (Subtype.mk hd h)
-        then
-          Except.ok (groundAtom.mk (Subtype.mk hd h) l p)
-        else Except.error ("relation arity does not match. Terms: " ++ listStringToString tl)
-      | Except.error msg => Except.error msg
-    else Except.error (hd ++ " is not a relation symbol")
+      if p:tl.length = (parsingSignature helper).relationArity (Subtype.mk hd h)
+      then
+        Except.ok {symbol:= Subtype.mk hd h, atom_terms := tl, term_length := p}
+      else
+        Except.error ("Wrong arity for symbol " ++ hd)
+    else Except.error ("Unknown symbol " ++ hd)
 
 
-def parseGroundAtom.go (relationList: List (String × Nat)) (l: List String) (stack: List String): Except String (groundAtom (parsingSignature relationList)) :=
+def parseGroundAtom.go (helper: parsingArityHelper) (l: List String) (stack: List String): Except String (groundAtom (parsingSignature helper)) :=
   match l with
   | List.nil => Except.error "No closing bracket"
   | hd::tl =>
     if hd == "("
-    then parseGroundAtom.go relationList tl stack
+    then parseGroundAtom.go helper tl stack
     else
       if hd == ")"
       then  if tl.isEmpty
-            then parseGroundAtomFromStack  relationList stack
+            then parseGroundAtomFromStack helper stack
             else Except.error "Symbols after the closing bracket when parsing atom"
       else
-        parseGroundAtom.go relationList tl (stack.append [hd])
+        parseGroundAtom.go helper tl (stack.append [hd])
 
-def parseGroundAtom (relationList: List (String × Nat)) (l: List String): Except String (groundAtom (parsingSignature relationList)) := parseGroundAtom.go relationList l []
+def parseGroundAtom (helper: parsingArityHelper) (l: List String):  Except String (groundAtom (parsingSignature helper)) := parseGroundAtom.go helper l []
 
 
-def proofTreeFromTree (relationList: List (String × Nat)) (t: Tree) : Except String (proofTree (parsingSignature relationList)) :=
+def proofTreeFromTree (helper: parsingArityHelper) (t: jsonTree) : Except String (proofTree (parsingSignature helper)) :=
   match t with
-  | Tree.node label children =>
-    match parseGroundAtom relationList (tokenize label) with
+  | jsonTree.node label children =>
+    match parseGroundAtom helper (tokenize label) with
     | Except.ok a =>
-      let s:= List.map_except (fun ⟨x, _h⟩  => proofTreeFromTree  relationList x) children.attach
+      let s:= List.map_except (fun ⟨x, _h⟩  => proofTreeFromTree  helper x) children.attach
       match s with
       | Except.ok l =>
         Except.ok (proofTree.node a l)
@@ -271,3 +215,16 @@ decreasing_by
   simp_wf
   decreasing_trivial
   apply Nat.zero_le
+
+structure verificationProblem (helper: parsingArityHelper) where
+  (trees: List (proofTree (parsingSignature helper)))
+  (program: List (rule (parsingSignature helper)))
+  (completion: Bool)
+
+def converProblemInputToVerificationProblem (helper: parsingArityHelper) (input: problemInput) : Except String (verificationProblem helper) :=
+  match List.map_except (proofTreeFromTree helper) input.trees with
+  | Except.error e => Except.error ("Error parsing trees -- " ++ e)
+  | Except.ok trees =>
+    match List.map_except (transformMockRuleToRule helper) input.program with
+    | Except.error e => Except.error ("Error parsing program -- " ++ e)
+    | Except.ok program => Except.ok {trees := trees, program := program, completion := input.completion}
